specs/L2AssetRouter/L2AssetRouter/Common/if_9037085336587543485_user.lean
@@ -14,12 +14,13 @@ section
 
 open Clear EVMState Ast Expr Stmt FunctionDefinition State Interpreter ExecLemmas OutOfFuelLemmas Abstraction YulNotation PrimOps ReasoningPrinciple Utilities L2AssetRouter.Common generated.L2AssetRouter L2AssetRouter
 
-def A_if_9037085336587543485 (s₀ s₉ : State) : Prop := sorry
+def A_if_9037085336587543485 (s₀ s₉ : State) : Prop := if_9037085336587543485_concrete_of_code.1 s₀ s₉
 
 lemma if_9037085336587543485_abs_of_concrete {s₀ s₉ : State} :
   Spec if_9037085336587543485_concrete_of_code s₀ s₉ →
   Spec A_if_9037085336587543485 s₀ s₉ := by
-  sorry
+  intro h
+  simpa [A_if_9037085336587543485] using h
 
 end
 
