specs/L2AssetRouter/L2AssetRouter/Common/switch_4568778344009629408_user.lean
@@ -25,12 +25,13 @@ section
 
 open Clear EVMState Ast Expr Stmt FunctionDefinition State Interpreter ExecLemmas OutOfFuelLemmas Abstraction YulNotation PrimOps ReasoningPrinciple Utilities L2AssetRouter.Common generated.L2AssetRouter L2AssetRouter
 
-def A_switch_4568778344009629408 (s₀ s₉ : State) : Prop := sorry
+def A_switch_4568778344009629408 (s₀ s₉ : State) : Prop := switch_4568778344009629408_concrete_of_code.1 s₀ s₉
 
 lemma switch_4568778344009629408_abs_of_concrete {s₀ s₉ : State} :
   Spec switch_4568778344009629408_concrete_of_code s₀ s₉ →
   Spec A_switch_4568778344009629408 s₀ s₉ := by
-  sorry
+  intro h
+  simpa [A_switch_4568778344009629408] using h
 
 end
 
