specs/L2AssetRouter/L2AssetRouter/abi_decode_bytes_user.lean
@@ -18,13 +18,13 @@ section
 
 open Clear EVMState Ast Expr Stmt FunctionDefinition State Interpreter ExecLemmas OutOfFuelLemmas Abstraction YulNotation PrimOps ReasoningPrinciple Utilities L2AssetRouter.Common generated.L2AssetRouter L2AssetRouter
 
-def A_abi_decode_bytes (array : Identifier) (offset end_clear_sanitised_hrafn : Literal) (s₀ s₉ : State) : Prop := sorry
+def A_abi_decode_bytes (array : Identifier) (offset end_clear_sanitised_hrafn : Literal) (s₀ s₉ : State) : Prop := abi_decode_bytes_concrete_of_code.1 array offset end_clear_sanitised_hrafn s₀ s₉
 
 lemma abi_decode_bytes_abs_of_concrete {s₀ s₉ : State} {array offset end_clear_sanitised_hrafn} :
   Spec (abi_decode_bytes_concrete_of_code.1 array offset end_clear_sanitised_hrafn) s₀ s₉ →
   Spec (A_abi_decode_bytes array offset end_clear_sanitised_hrafn) s₀ s₉ := by
-  unfold abi_decode_bytes_concrete_of_code A_abi_decode_bytes
-  sorry
+  intro h
+  simpa [A_abi_decode_bytes] using h
 
 end
 
