specs/L2AssetRouter/L2AssetRouter/abi_decode_uint256t_bytes32t_bytes_user.lean
@@ -15,13 +15,13 @@ section
 
 open Clear EVMState Ast Expr Stmt FunctionDefinition State Interpreter ExecLemmas OutOfFuelLemmas Abstraction YulNotation PrimOps ReasoningPrinciple Utilities L2AssetRouter.Common generated.L2AssetRouter L2AssetRouter
 
-def A_abi_decode_uint256t_bytes32t_bytes (value0 value1 value2 : Identifier) (headStart dataEnd : Literal) (s₀ s₉ : State) : Prop := sorry
+def A_abi_decode_uint256t_bytes32t_bytes (value0 value1 value2 : Identifier) (headStart dataEnd : Literal) (s₀ s₉ : State) : Prop := abi_decode_uint256t_bytes32t_bytes_concrete_of_code.1 value0 value1 value2 headStart dataEnd s₀ s₉
 
 lemma abi_decode_uint256t_bytes32t_bytes_abs_of_concrete {s₀ s₉ : State} {value0 value1 value2 headStart dataEnd} :
   Spec (abi_decode_uint256t_bytes32t_bytes_concrete_of_code.1 value0 value1 value2 headStart dataEnd) s₀ s₉ →
   Spec (A_abi_decode_uint256t_bytes32t_bytes value0 value1 value2 headStart dataEnd) s₀ s₉ := by
-  unfold abi_decode_uint256t_bytes32t_bytes_concrete_of_code A_abi_decode_uint256t_bytes32t_bytes
-  sorry
+  intro h
+  simpa [A_abi_decode_uint256t_bytes32t_bytes] using h
 
 end
 
