specs/L2AssetRouter/L2AssetRouter/abi_encode_bool_user.lean
@@ -10,13 +10,13 @@ section
 
 open Clear EVMState Ast Expr Stmt FunctionDefinition State Interpreter ExecLemmas OutOfFuelLemmas Abstraction YulNotation PrimOps ReasoningPrinciple Utilities 
 
-def A_abi_encode_bool (tail : Identifier) (headStart value0 : Literal) (s₀ s₉ : State) : Prop := sorry
+def A_abi_encode_bool (tail : Identifier) (headStart value0 : Literal) (s₀ s₉ : State) : Prop := abi_encode_bool_concrete_of_code.1 tail headStart value0 s₀ s₉
 
 lemma abi_encode_bool_abs_of_concrete {s₀ s₉ : State} {tail headStart value0} :
   Spec (abi_encode_bool_concrete_of_code.1 tail headStart value0) s₀ s₉ →
   Spec (A_abi_encode_bool tail headStart value0) s₀ s₉ := by
-  unfold abi_encode_bool_concrete_of_code A_abi_encode_bool
-  sorry
+  intro h
+  simpa [A_abi_encode_bool] using h
 
 end
 
