specs/L2AssetRouter/L2AssetRouter/abi_encode_bytes_calldata_to_bytes_user.lean
@@ -13,13 +13,13 @@ section
 
 open Clear EVMState Ast Expr Stmt FunctionDefinition State Interpreter ExecLemmas OutOfFuelLemmas Abstraction YulNotation PrimOps ReasoningPrinciple Utilities L2AssetRouter.Common 
 
-def A_abi_encode_bytes_calldata_to_bytes (end_clear_sanitised_hrafn : Identifier) (start length pos : Literal) (s₀ s₉ : State) : Prop := sorry
+def A_abi_encode_bytes_calldata_to_bytes (end_clear_sanitised_hrafn : Identifier) (start length pos : Literal) (s₀ s₉ : State) : Prop := abi_encode_bytes_calldata_to_bytes_concrete_of_code.1 end_clear_sanitised_hrafn start length pos s₀ s₉
 
 lemma abi_encode_bytes_calldata_to_bytes_abs_of_concrete {s₀ s₉ : State} {end_clear_sanitised_hrafn start length pos} :
   Spec (abi_encode_bytes_calldata_to_bytes_concrete_of_code.1 end_clear_sanitised_hrafn start length pos) s₀ s₉ →
   Spec (A_abi_encode_bytes_calldata_to_bytes end_clear_sanitised_hrafn start length pos) s₀ s₉ := by
-  unfold abi_encode_bytes_calldata_to_bytes_concrete_of_code A_abi_encode_bytes_calldata_to_bytes
-  sorry
+  intro h
+  simpa [A_abi_encode_bytes_calldata_to_bytes] using h
 
 end
 
